tests/bitfields/Test.fst
@@ -51,11 +51,27 @@ let reserved_bits : enum unit (bitfield uint8 2) = [
   (), 0uy;
 ]
 
+open LowParse.Spec.BoundedInt
+
+inline_for_extraction
+noextract
+type packet_number_length_t = bounded_int32 1 4
+
+[@filter_bitsum'_t_attr]
+inline_for_extraction
+noextract
+let packet_number_length : enum packet_number_length_t (bitfield uint8 2) = [
+  1ul, 0uy;
+  2ul, 1uy;
+  3ul, 2uy;
+  4ul, 3uy;
+]
+
 [@filter_bitsum'_t_attr]
 inline_for_extraction
 noextract
 let rrpp : bitsum' uint8 4 =
-  BitSum' _ _ reserved_bits (fun _ -> BitField 2 (BitStop ()))
+  BitSum' _ _ reserved_bits (fun _ -> BitSum' _ _ packet_number_length (fun _ -> BitStop ()))
 
 [@filter_bitsum'_t_attr]
 inline_for_extraction
@@ -98,6 +114,27 @@ let f (x: FStar.UInt8.t) : Tot unit =
     T.norm [primops; iota; zeta; delta_attr [`%filter_bitsum'_t_attr]];
     T.fail "abc"
   )
+*)
+
+open LowParse.Spec.Bytes
+open LowParse.Spec.DepLen
+
+module FB = FStar.Bytes
+
+noeq
+type common_long_message = {
+  version: FB.lbytes 4;
+  dcid: parse_bounded_vlbytes_t 0 255;
+  scid: parse_bounded_vlbytes_t 0 255;
+}
+
+(*
+noeq
+type long_message =
+| MZeroRTT:
+  (common: common_long_message) ->
+  (packet_number: parse_bounded_vlbytes_t 1 4) ->
+  (payload: parse_bounded_vlbytes_t 0 63) ->
 *)
 
 let main
