.docker/build/build.sh
@@ -76,6 +76,7 @@ function raise () {
 
 function build_and_test_quackyducky() {
     fetch_and_make_kremlin &&
+    export_home QD "$(pwd)" &&
     make -j $threads -k test &&
     # Build incrementality test
     pushd tests/sample && {
